tearing apart Rtac and putting it back together
1) Substitutions are now built into Goal.
   - in the future, can we substitute away instantiated terms?
2) runRTac is the main way to execute tactics
   - it is *not* very efficient though
   - too much goal manipulation, even on simple combinators like THEN
   - Is it possible to CPS convert the entire thing?
3) A likely buggy version of rtac_sound
4) Conjunctions in goals
5) Eliminate Open, that is now part of Core.

theories/RTac/Core.v
@@ -1,5 +1,7 @@
 Require Import ExtLib.Structures.Monad.
 Require Import ExtLib.Structures.Traversable.
+Require Import ExtLib.Data.Prop.
+Require Import ExtLib.Data.List.
 Require Import ExtLib.Data.Monads.OptionMonad.
 Require Import ExtLib.Tactics.
 Require Import MirrorCore.EnvI.
@@ -7,53 +9,187 @@ Require Import MirrorCore.ExprI.
 Require Import MirrorCore.TypesI.
 Require Import MirrorCore.SubstI.
 Require Import MirrorCore.ExprDAs.
-Require Import MirrorCore.STac.Core.
 
 Require Import MirrorCore.Util.Forwardy.
 
 Set Implicit Arguments.
 Set Strict Implicit.
 
-(** TODO: Can I do alternation if I can do strengthening of both
- ** unification variables and regular variables?
- ** 1) This means that substD needs strengthening
- ** 2) It also means that hypotheses need to be eliminatable
- **
- **    goal :=
- **      Alls : list typ -> goal -> goal
- **    | Exs : list typ -> goal -> goal
- **    | Hyps : list expr -> goal -> goal
- **    | Goal : expr -> goal.
- **
- **)
 Section parameterized.
   Variable typ : Type.
   Variable expr : Type.
   Variable subst : Type.
-
-  (** NOTE: It seems for performance this should be inverted, otherwise
-   ** every operation is going to be very expensive.
-   **)
-  Inductive Goal :=
-  | GAlls : typ -> Goal -> Goal
-  | GExs  : typ -> Goal -> Goal
-  | GHyps : expr -> Goal -> Goal
-  | GGoal : subst -> option expr -> Goal.
-
-  Definition Result := option Goal.
-
-  (** Treat this as opaque! **)
-  Definition rtac : Type :=
-    Goal -> Result.
-
-  Definition runRTac (tac : rtac) (g : Goal) : option Goal :=
-    tac g.
 
   Context {RType_typ : RType typ}.
   Context {Expr_expr : Expr RType_typ expr}.
   Context {Typ0_Prop : Typ0 _ Prop}.
   Context {Subst_subst : Subst subst expr}.
   Context {SubstOk_subst : @SubstOk _ _ _ _ Expr_expr Subst_subst}.
+  Context {SubstUpdate_subst : SubstUpdate subst expr}.
+  Context {SubstUpdateOk_subst : @SubstUpdateOk _ _ _ _ Expr_expr Subst_subst _ _}.
+
+
+  (** NOTE: It seems for performance this should be inverted, otherwise
+   ** every operation is going to be expensive.
+   **)
+  Inductive Goal :=
+  | GAll    : typ -> Goal -> Goal
+  (** The first thing in the list has the lowest index **)
+  | GExs    : list (typ * option expr) -> Goal -> Goal
+  | GHyp    : expr -> Goal -> Goal
+  | GConj   : list Goal -> Goal
+  | GGoal   : expr -> Goal
+  | GSolved : Goal.
+
+  Definition GAlls (ts : list typ) (g : Goal) : Goal :=
+    fold_right (fun x y => GAll x y) g ts.
+
+  Definition GEx (t : typ) (e : option expr) (g : Goal) : Goal :=
+    match g with
+      | GExs tes g' => GExs (tes ++ (t,e) :: nil) g'
+      | _ => GExs ((t, e) :: nil) g
+    end.
+
+  Inductive Ctx :=
+  | CTop
+  | CAll : Ctx -> typ -> Ctx
+  | CEx  : Ctx -> typ -> Ctx
+  | CHyp : Ctx -> expr -> Ctx.
+
+  (** StateT subst Option Goal **)
+  Inductive Result :=
+  | Fail
+  | More   : subst -> Goal -> Result
+  | Solved : subst -> Result.
+
+  Definition DEAD : Result.
+    exact Fail.
+  Qed.
+
+  (** Treat this as opaque! **)
+  Definition rtac : Type :=
+    Ctx -> subst -> expr -> Result.
+
+  Fixpoint countVars' (ctx : Ctx) acc : nat :=
+    match ctx with
+      | CTop => acc
+      | CAll ctx' t => countVars' ctx' (S acc)
+      | CEx  ctx' _
+      | CHyp ctx' _ => countVars' ctx' acc
+    end.
+
+  Fixpoint countUVars' (ctx : Ctx) acc : nat :=
+    match ctx with
+      | CTop => acc
+      | CEx  ctx' t => countUVars' ctx' (S acc)
+      | CAll ctx' _
+      | CHyp ctx' _ => countUVars' ctx' acc
+    end.
+
+  Definition countVars ctx := countVars' ctx 0.
+  Definition countUVars ctx := countUVars' ctx 0.
+
+  Fixpoint getEnvs' (ctx : Ctx) (tus tvs : tenv typ)
+  : tenv typ * tenv typ :=
+    match ctx with
+      | CTop => (tus,tvs)
+      | CAll ctx' t => getEnvs' ctx' tus (t :: tvs)
+      | CEx  ctx' t => getEnvs' ctx' (t :: tus) tvs
+      | CHyp ctx' _ => getEnvs' ctx' tus tvs
+    end.
+
+  Definition getEnvs (ctx : Ctx) : tenv typ * tenv typ :=
+    let (x,y) := getEnvs' ctx nil nil in
+    (x, y).
+
+  Definition mapUnderEx (t : typ) (nus : nat) (r : Result) : Result :=
+    match r with
+      | Fail => Fail
+      | Solved s' =>
+        match lookup nus s' with
+          | None => let s'' := s' in
+                    More s'' (GEx t None GSolved)
+          | Some e =>
+            match drop nus s' with
+              | None => DEAD
+              | Some s'' => Solved s''
+            end
+        end
+      | More s' g' =>
+        match lookup nus s' with
+          | None => let s'' := s' in
+                    More s' (GEx t None g')
+          | Some e =>
+            match drop nus s' with
+              | None => DEAD
+              | Some s'' => More s'' (GEx t (Some e) g')
+            end
+        end
+    end.
+
+  Section runRTac'.
+    Variable tac : rtac.
+
+    Fixpoint runRTac' (ctx : Ctx) (s : subst) (g : Goal) (nus nvs : nat) {struct g}
+    : Result :=
+      match g with
+        | GGoal e => tac ctx s e
+        | GSolved => Solved s
+        | GAll t g =>
+          match runRTac' (CAll ctx t) s g nus (S nvs) with
+            | Fail => Fail
+            | Solved s => Solved s
+            | More s g => More s (GAll t g)
+          end
+        | GExs tes g =>
+          (fix go (nus : nat) (tes : list (typ * option expr)) (s : subst) (ctx : Ctx)
+           : Result :=
+             match tes with
+               | nil => runRTac' ctx s g nus nvs
+               | (t,e) :: tes =>
+                 match e with
+                   | None =>
+                     mapUnderEx t nus (runRTac' (CEx ctx t) s g (S nus) nvs)
+                   | Some e' =>
+                     match set nus e' s with
+                       | None => DEAD
+                       | Some s' =>
+                         mapUnderEx t nus (runRTac' (CEx ctx t) s' g (S nus) nvs)
+                     end
+                 end
+             end) nus tes s ctx
+        | GHyp h g =>
+          match runRTac' (CHyp ctx h) s g nus nvs with
+            | Fail => Fail
+            | Solved s => Solved s
+            | More s g => More s (GHyp h g)
+          end
+        | GConj gs =>
+          (fix do_each (gs : list Goal) (s : subst)
+               (acc : list Goal -> subst -> Result)
+           : Result :=
+             match gs with
+               | nil => acc nil s
+               | g :: gs =>
+                 match runRTac' ctx s g nus nvs with
+                   | Fail => Fail
+                   | Solved s => do_each gs s acc
+                   | More s g =>
+                     do_each gs s (fun other s => acc (g :: other) s)
+                 end
+             end) gs s
+                  (fun rem s =>
+                     match rem with
+                       | nil => Solved s
+                       | _ :: _ => More s (GConj rem)
+                     end)
+      end.
+
+    Definition runRTac (ctx : Ctx) (s : subst) (g : Goal)
+    : Result :=
+      runRTac' ctx s g (countUVars ctx) (countVars ctx).
+  End runRTac'.
+
 
   Definition propD := @exprD'_typ0 _ _ _ _ Prop _.
 
@@ -79,35 +215,115 @@ Section parameterized.
       | l :: ls => l -> _impls ls P
     end.
 
-  Fixpoint WellFormed_goal (goal : Goal) : Prop :=
+  Section _and.
+    Context {A B : Type}.
+    Variables (a : A) (b : B).
+    Fixpoint _and (ls : list (A -> B -> Prop)) :=
+      match ls with
+        | nil => True
+        | l :: nil => l a b
+        | l :: ls => l a b /\ _and ls
+      end.
+  End _and.
+
+  (** TODO: I hope that there is a better way to reason about this **)
+  Inductive Path (f : nat -> nat -> Prop) : nat -> nat -> Prop :=
+  | PDirect : forall x y, f x y -> Path f x y
+  | PThrough : forall x y z, f x y -> Path f y z -> Path f x z.
+
+  Definition Acyclic_from (tus tvs : nat) (tes : list (typ * option expr))
+  : Prop :=
+    (forall x, ~Path (fun f t =>
+                        f > tus /\ t > tus /\
+                        exists z e,
+                          nth_error tes (f - tus) = Some (z, Some e) /\
+                          mentionsU t e = true) x x) /\
+    (forall t e, In (t,Some e) tes ->
+                 forall u, mentionsU u e = true ->
+                           u < tus + length tes).
+
+  (** Well_formedness is about acyclicity, but we don't have enough now
+   ** to guarantee that.
+   ** We could make a acyclic judgement on a map and just construct the map.
+   ** Either way things are getting a lot more complex here than I wanted them
+   ** too.
+   **)
+  Fixpoint WellFormed_goal (tus tvs : nat) (goal : Goal) : Prop :=
     match goal with
-      | GAlls _ goal'
-      | GExs _ goal'
-      | GHyps _ goal' => WellFormed_goal goal'
-      | GGoal s _ => WellFormed_subst s
+      | GAll _ goal' => WellFormed_goal tus (S tvs) goal'
+      | GExs tes goal' =>
+           Acyclic_from tus tvs tes
+        /\ WellFormed_goal (tus + length tes) tvs goal'
+      | GHyp _ goal' => WellFormed_goal tus tvs goal'
+      | GGoal _ => True
+      | GSolved => True
+      | GConj ls =>
+        (fix Forall (ls : list Goal) : Prop :=
+           match ls with
+             | nil => True
+             | l :: ls => WellFormed_goal tus tvs l /\ Forall ls
+           end) ls
     end.
+
+  Fixpoint hlist_mapT {T : Type} {F : T -> Type}
+           {ls : list T} (h : HList.hlist (fun x => option (F x)) ls)
+  : option (HList.hlist F ls) :=
+    match h in HList.hlist _ ls return option (HList.hlist F ls) with
+      | HList.Hnil => Some (HList.Hnil)
+      | HList.Hcons _ _ x y =>
+        match x , hlist_mapT y with
+          | Some x , Some y => Some (HList.Hcons x y)
+          | _ , _ => None
+        end
+    end.
+
+  Fixpoint goal_substD (tus tvs : list typ) (tes : list (typ * option expr))
+  : ResType (tus ++ map fst tes) tvs Prop.
+(*
+  refine
+    match tes as tes return ResType (tus ++ map fst tes) tvs Prop with
+      | nil => Some (fun _ _ => True)
+      | (t,None) :: tes =>
+        goal_substD (tus ++ t :: nil) tvs tes
+      | (t,Some e) :: tes =>
+        match exprD' tus tvs e t
+            , goal_substD tus tvs tes
+        with
+          | Some eD , Some sD => _
+          | _ , _ => None
+        end
+    end.
+*)
+  Admitted.
 
   (** NOTE:
    ** Appending the newly introduced terms makes tactics non-local.
-   ** Requiring globalness seems really bad.
+   ** Requiring globalness seems bad.
+   ** - The alternative, however, is to expose a lot more operations
+   **   on substitute
    **)
-  Fixpoint goalD (tus tvs : list typ) (goal : Goal)
-  : ResType tus tvs Prop :=
+  Fixpoint goalD (tus tvs : list typ) (goal : Goal) {struct goal}
+  : ResType tus tvs Prop.
+  refine
     match goal with
-      | GAlls tv goal' =>
+      | GAll tv goal' =>
         match goalD tus (tvs ++ tv :: nil) goal' with
           | None => None
           | Some D =>
             Some (fun us vs => @_foralls (tv :: nil) (fun vs' => D us (HList.hlist_app vs vs')))
         end
-      | GExs tu goal' =>
-        match goalD (tus ++ tu :: nil) tvs goal' with
-          | None => None
-          | Some D =>
-            Some (fun us vs => @_exists (tu :: nil)
-                      (fun us' => D (HList.hlist_app us us') vs))
+      | GExs tes goal' =>
+        let tus_ext := map fst tes in
+        match goalD (tus ++ tus_ext) tvs goal'
+            , goal_substD tus tvs tes with
+          | None , _ => None
+          | Some _ , None => None
+          | Some D , Some sD =>
+            Some (fun us vs => @_exists tus_ext
+                                        (fun us' => sD (HList.hlist_app us us') vs
+                                                    /\ D (HList.hlist_app us us') vs))
         end
-      | GHyps hyp' goal' =>
+      | GHyp hyp' goal' =>
         match mapT (T:=list) (F:=option) (propD tus tvs) (hyp' :: nil) with
           | None => None
           | Some hs =>
@@ -117,41 +333,124 @@ Section parameterized.
                 Some (fun us vs => _impls (map (fun x => x us vs) hs) (D us vs))
             end
         end
-      | GGoal sub' None =>
-        match substD tus tvs sub' with
-          | Some sD => Some (fun us vs => sD us vs)
-          | _ => None
+      | GConj ls =>
+        (** This is actually:
+        match mapT (T:=list) (F:=option) (goalD tus tvs) ls with
+          | None => None
+          | Some lD =>
+            Some (fun us vs => _and us vs lD)
         end
-      | GGoal sub' (Some goal') =>
-        match substD tus tvs sub'
-            , propD tus tvs goal'
-        with
-          | Some sD , Some gD =>
-            Some (fun (us : HList.hlist typD tus)
-                      (vs : HList.hlist typD tvs)  => sD us vs /\ gD us vs)
-          | _ , _ => None
+        **)
+        match mapT_list (F:=option) (goalD tus tvs) ls with
+          | None => None
+          | Some lD => Some (fun us vs => _and us vs lD)
         end
+      | GSolved => Some (fun _ _ => True)
+      | GGoal goal' => propD tus tvs goal'
     end.
+  Defined.
 
-  (** The worry is that this isn't going to be strong enough,
-   ** especially when it comes to substitutions.
-   **)
-  Definition rtac_sound tus tvs (tac : rtac) : Prop :=
-    forall g g',
-      tac g = Some g' ->
-      WellFormed_goal g ->
-      WellFormed_goal g' /\
-      match goalD tus tvs g
-          , goalD tus tvs g'
-      with
-        | None , _ => True
-        | Some _ , None => False
-        | Some g , Some g' =>
-          forall us vs,
-            g' us vs ->
-            g us vs
+  Definition OpenT (tus tvs : tenv typ) (T : Type) : Type :=
+    HList.hlist typD tus -> HList.hlist typD tvs -> T.
+
+  Section ctxD.
+    Variable P : forall (tus' tvs' : tenv typ),
+                   unit + option (OpenT tus' tvs' Prop).
+
+
+    Fixpoint ctxD (tus tvs : tenv typ) (ctx : Ctx) {struct ctx}
+    : unit + option (OpenT tus tvs Prop) :=
+      match ctx with
+        | CTop => P tus tvs
+        | CEx ctx' t =>
+          match ctxD (tus ++ t :: nil) tvs ctx' with
+            | inr (Some PD) =>
+              (** The [forall] here is on purpose, [ctxD] is used to construct
+               ** holes and in holes, everything is a variable
+               **)
+              inr (Some (fun us vs => forall x : typD t,
+                           PD (HList.hlist_app us (HList.Hcons x HList.Hnil))
+                              vs))
+            | inl x => inl x
+            | inr None => inr None
+          end
+        | CAll ctx' t =>
+          match ctxD tus (tvs ++ t :: nil) ctx' with
+            | inr (Some PD) =>
+              inr (Some (fun us vs => forall x : typD t,
+                           PD us
+                              (HList.hlist_app vs (HList.Hcons x HList.Hnil))))
+            | inl x => inl x
+            | inr None => inr None
+          end
+        | CHyp ctx' h =>
+          match propD tus tvs h with
+            | None => inl tt
+            | Some hD =>
+              match ctxD tus tvs ctx' with
+                | inr (Some PD) =>
+                  inr (Some (fun us vs => hD us vs -> PD us vs))
+                | inl x => inl x
+                | inr None => inr None
+              end
+          end
+      end.
+  End ctxD.
+
+  Definition rtac_sound (tus tvs : tenv typ) (tac : rtac) : Prop :=
+    forall ctx s g result,
+      tac ctx s g = result ->
+      match result with
+        | Fail => True
+        | Solved s' =>
+          WellFormed_subst s ->
+          WellFormed_subst s' /\
+          match ctxD (fun tus' tvs' =>
+                        match propD tus' tvs' g
+                            , substD tus' tvs' s
+                            , substD tus' tvs' s'
+                        with
+                          | None , _ , _ => inl tt
+                          | Some _ , None , _ => inl tt
+                          | Some _ , Some _ , None => inr None
+                          | Some gD , Some sD , Some sD' =>
+                            inr (Some (fun us vs =>
+                                         sD' us vs ->
+                                         sD us vs /\ gD us vs))
+                        end)
+                     tus tvs ctx
+          with
+            | inl _ => True
+            | inr None => False
+            | inr (Some gD) => forall us vs, gD us vs
+          end
+        | More s' g' =>
+          WellFormed_subst s ->
+          WellFormed_subst s' /\
+          match ctxD (fun tus' tvs' =>
+                        match propD tus' tvs' g
+                            , substD tus' tvs' s
+                            , goalD tus' tvs' g'
+                            , substD tus' tvs' s'
+                        with
+                          | None , _ , _ , _
+                          | Some _ , None , _ , _ => inl tt
+                          | Some _ , Some _ , None , _
+                          | Some _ , Some _ , Some _ , None => inr None
+                          | Some gD , Some sD , Some gD' , Some sD' =>
+                            inr (Some (fun us vs =>
+                                         sD' us vs -> gD' us vs ->
+                                         sD us vs /\ gD us vs))
+                        end)
+                     tus tvs ctx
+          with
+            | inl _ => True
+            | inr None => False
+            | inr (Some gD) => forall us vs, gD us vs
+          end
       end.
 
+(*
   Section at_bottom.
     Variable m : Type -> Type.
     Context {Monad_m : Monad m}.
@@ -162,13 +461,13 @@ Section parameterized.
 
     Fixpoint at_bottom tus tvs (g : Goal) : m Goal :=
       match g with
-        | GAlls x g' => under (GAlls x) (at_bottom tus (tvs ++ x :: nil) g')
-        | GExs  x g' => under (GExs  x) (at_bottom (tus ++ x :: nil) tvs g')
-        | GHyps x g' => under (GHyps x) (at_bottom tus tvs g')
+        | GAll x g' => under (GAll x) (at_bottom tus (tvs ++ x :: nil) g')
+        | GEx  x g' => under (GEx  x) (at_bottom (tus ++ x :: nil) tvs g')
+        | GHyp x g' => under (GHyp x) (at_bottom tus tvs g')
         | GGoal s e => gt tus tvs s e
       end.
   End at_bottom.
-
+*)
   Lemma goalD_conv
   : forall tus tvs tus' tvs' (pfu : tus' = tus) (pfv : tvs' = tvs),
       goalD tus tvs =
@@ -216,6 +515,7 @@ Section parameterized.
       intro; eapply H.
   Qed.
 
+(*
   Lemma at_bottom_sound_option
   : forall goal tus tvs f goal',
       (forall tus' tvs' s e e',
@@ -326,6 +626,7 @@ Section parameterized.
       repeat rewrite HList.app_nil_r_trans in H.
       eapply H in H0; clear H; auto. }
   Qed.
+*)
 
   Lemma _exists_sem : forall ls P,
                         _exists (ls := ls) P <->
@@ -363,6 +664,7 @@ Section parameterized.
         intros. eapply H.
   Qed.
 
+(*
   Lemma at_bottom_WF_option
   : forall f,
       (forall a b c d g,
@@ -377,28 +679,31 @@ Section parameterized.
     clear.
     induction g; simpl; intros; forwardy; inv_all; subst; simpl in *; eauto.
   Qed.
+*)
 
-  Lemma WellFormed_goal_GAlls
+(*
+  Lemma WellFormed_goal_GAll
   : forall ls g,
-      WellFormed_goal g <-> WellFormed_goal (fold_right GAlls g ls).
+      WellFormed_goal g <-> WellFormed_goal (fold_right GAll g ls).
   Proof.
     clear. induction ls; simpl; intros; auto.
     reflexivity.
   Qed.
-  Lemma WellFormed_goal_GExs
+  Lemma WellFormed_goal_GEx
   : forall ls g,
-      WellFormed_goal g <-> WellFormed_goal (fold_right GExs g ls).
+      WellFormed_goal g <-> WellFormed_goal (fold_right GEx g ls).
   Proof.
     clear. induction ls; simpl; intros; auto.
     reflexivity.
   Qed.
-  Lemma WellFormed_goal_GHyps
+  Lemma WellFormed_goal_GHyp
   : forall ls g,
-      WellFormed_goal g <-> WellFormed_goal (fold_right GHyps g ls).
+      WellFormed_goal g <-> WellFormed_goal (fold_right GHyp g ls).
   Proof.
     clear. induction ls; simpl; intros; auto.
     reflexivity.
   Qed.
+*)
 
 (*
   Instance Monad_writer_nat : Monad (fun T : Type => (T * nat)%type) :=
@@ -417,7 +722,7 @@ Section parameterized.
     fun g =>
       let (g',n) :=
           at_bottom (m := fun T => (T * nat))%type
-                    (fun tus _ s g => (GExs t (GGoal s g), length tus)) nil nil g
+                    (fun tus _ s g => (GEx t (GGoal s g), length tus)) nil nil g
       in
       k n g'.
 *)
@@ -431,16 +736,41 @@ Section parameterized.
   : rtac :=
     fun g =>
       let (g',uv) :=
-          at_bottom (fun _ tvs g => (GAlls t g, length tvs)) nil nil g
+          at_bottom (fun _ tvs g => (GAll t g, length tvs)) nil nil g
       in
       k uv g'.
 *)
 
+  (** NOTE: Probably not neccessary **)
+  Fixpoint closeGoal (ctx : Ctx) (s : subst) (g : Goal) (nus : nat)
+  : Goal :=
+    match ctx with
+      | CTop => g
+      | CAll c t => closeGoal c s (GAll t g) nus
+      | CEx  c t =>
+        closeGoal c s (GEx t (lookup nus s) g) (S nus)
+      | CHyp c h => closeGoal c s (GHyp h g) nus
+    end.
+
+
+
 End parameterized.
 
+(*
 Arguments propD {typ expr _ _ _} tus tvs e : rename.
-Arguments rtac_sound {typ expr subst _ _ _ _ _} tus tvs tac : rename.
-Arguments GExs {typ expr subst} _ _ : rename.
-Arguments GAlls {typ expr subst} _ _ : rename.
-Arguments GHyps {typ expr subst} _ _ : rename.
-Arguments GGoal {typ expr subst} _ _ : rename.
+Arguments rtac_sound {typ expr subst} tus tvs tac : rename.
+*)
+Arguments GEx {typ expr} _ _ _ : rename.
+Arguments GAll {typ expr} _ _ : rename.
+Arguments GHyp {typ expr} _ _ : rename.
+Arguments GConj {typ expr} _ : rename.
+Arguments GGoal {typ expr} _ : rename.
+Arguments GSolved {typ expr} : rename.
+Arguments CTop {typ expr} : rename.
+Arguments CEx {typ expr} _ _ : rename.
+Arguments CAll {typ expr} _ _ : rename.
+Arguments CHyp {typ expr} _ _ : rename.
+
+Arguments Fail {typ expr subst} : rename.
+Arguments More {typ expr subst} _ _ : rename.
+Arguments Solved {typ expr subst} _ : rename.
