theories/RTac/Instantiate.v
@@ -1,9 +1,11 @@
+Require Import ExtLib.Data.Sum.
 Require Import ExtLib.Tactics.
 Require Import MirrorCore.EnvI.
 Require Import MirrorCore.ExprI.
 Require Import MirrorCore.TypesI.
 Require Import MirrorCore.SubstI.
 Require Import MirrorCore.RTac.Core.
+Require Import MirrorCore.RTac.Simplify.
 
 Require Import MirrorCore.Util.Forwardy.
 
@@ -20,22 +22,18 @@ Section parameterized.
   Context {Subst_subst : Subst subst expr}.
   Context {SubstOk_subst : @SubstOk _ _ _ _ Expr_expr Subst_subst}.
 
-  Definition TRY (tac : rtac typ expr subst) : rtac typ expr subst :=
-    fun ctx s g => match tac ctx s g with
-                     | Fail => More s (GGoal g)
-                     | x => x
-                   end.
+  Variable instantiate : (nat -> option expr) -> nat -> expr -> expr.
 
-  Theorem TRY_sound
-  : forall tus tvs tac, rtac_sound tus tvs tac -> rtac_sound tus tvs (TRY tac).
+  Section instantiate.
+    Definition INSTANTIATE
+    : rtac typ expr subst :=
+      @SIMPLIFY typ expr subst
+                (fun _ sub => instantiate (fun u => lookup u sub) 0).
+  End instantiate.
+
+  Theorem INSTANTIATE_sound
+  : forall tus tvs, rtac_sound tus tvs INSTANTIATE.
   Proof.
-    unfold TRY, rtac_sound.
-    intros; subst.
-    specialize (H ctx s g _ eq_refl).
-    destruct (tac ctx s g); auto.
-    + intros; split; auto.
-      simpl.
-      admit.
-  Qed.
+  Admitted.
 
 End parameterized.
