theories/RTac/Apply.v
@@ -5,12 +5,11 @@ Require Import MirrorCore.ExprI.
 Require Import MirrorCore.TypesI.
 Require Import MirrorCore.SubstI.
 Require Import MirrorCore.ExprDAs.
-Require Import MirrorCore.RTac.Core.
 Require Import MirrorCore.Lemma.
-Require Import MirrorCore.RTac.Continuation.
-Require Import MirrorCore.RTac.Open.
 Require Import MirrorCore.LemmaApply.
 Require Import MirrorCore.InstantiateI.
+Require Import MirrorCore.RTac.Core.
+Require Import MirrorCore.RTac.Reduce.
 
 Require Import MirrorCore.Util.Forwardy.
 
@@ -22,13 +21,13 @@ Section parameterized.
   Variable expr : Type.
   Variable subst : Type.
 
-  Variable RType_typ : RType typ.
-  Variable Expr_expr : Expr RType_typ expr.
-  Variable Typ0_Prop : Typ0 _ Prop.
-  Variable Subst_subst : Subst subst expr.
-  Variable SubstOk_subst : @SubstOk _ _ _ _ Expr_expr Subst_subst.
-  Variable SU : SubstUpdate subst expr.
-  Variable SubstUpdateOk_subst : @SubstUpdateOk _ _ _ _ Expr_expr Subst_subst _ _.
+  Context {RType_typ : RType typ}.
+  Context {Expr_expr : Expr RType_typ expr}.
+  Context {Typ0_Prop : Typ0 _ Prop}.
+  Context {Subst_subst : Subst subst expr}.
+  Context {SubstOk_subst : @SubstOk _ _ _ _ Expr_expr Subst_subst}.
+  Context {SU : SubstUpdate subst expr}.
+  Context {SubstUpdateOk_subst : @SubstUpdateOk _ _ _ _ Expr_expr Subst_subst _ _}.
 
   Variable vars_to_uvars : nat -> nat -> expr -> expr.
   Variable exprUnify :
@@ -39,67 +38,26 @@ Section parameterized.
     @eapplicable typ _ expr _ subst vars_to_uvars
                  exprUnify.
 
-  Section fm2.
-    Variable T U V : Type.
-    Variable f : T -> U -> option V.
-    Fixpoint filter_map2 (ls : list T) (ls' : list U) : option (list V) :=
-      match ls , ls' with
-        | nil , nil => Some nil
-        | l :: ls , l' :: ls' =>
-          match f l l' with
-            | None => filter_map2 ls ls'
-            | Some x => match filter_map2 ls ls' with
-                          | None => None
-                          | Some xs => Some (x :: xs)
-                        end
-          end
-        | _ , _ => None
-      end.
-  End fm2.
-
-  Fixpoint all_success (f : expr -> subst -> option (Goal typ expr subst))
-           (sub : _) (ls : list expr)
-  : option (Goal typ expr subst) :=
-    match ls with
-      | nil => Some (GGoal sub None)
-      | l :: ls =>
-        match f l sub with
-          | None => None
-          | Some (GGoal sub' None) => all_success f sub' ls
-          | Some x =>
-            match ls with
-              | nil => Some x
-              | _ :: _ => None
-            end
-        end
-    end.
-
   Definition APPLY
              (lem : Lemma.lemma typ expr expr)
-             (tacC : rtac_cont typ expr subst)
   : rtac typ expr subst :=
     let len_vars := length lem.(vars) in
-    fun gl =>
-      let '(ctx,sub,goal) := openGoal gl in
-      match goal with
-        | None => Some gl
-        | Some goal =>
-          let '(tus,tvs) := getEnvs ctx in
-          match eapplicable sub tus tvs lem goal with
-            | None => None
-            | Some sub' =>
-              let len_uvars := length tus in
-              match pull (expr := expr) (SU := SU) len_uvars len_vars sub' with
-                | Some sub'' =>
-                  let premises :=
-                      map (fun e => instantiate (fun u => lookup u sub') 0
-                                                (vars_to_uvars 0 len_uvars e))
-                          lem.(premises)
-                  in
-                  (** Solve the side conditions **)
-                  tacC ctx sub premises
-                | None => None
-              end
+    fun ctx sub goal =>
+      let '(tus,tvs) := getEnvs ctx in
+      match eapplicable sub tus tvs lem goal with
+        | None => Fail
+        | Some sub' =>
+          let len_uvars := length tus in
+          match pull (expr := expr) (SU := SU) len_uvars len_vars sub' with
+            | Some sub'' =>
+              let premises :=
+                  map (fun e => instantiate (fun u => lookup u sub') 0
+                                            (vars_to_uvars 0 len_uvars e))
+                      lem.(premises)
+              in
+              more_list instantiate CTop sub'' (map GGoal premises)
+              (** Solve the side conditions **)
+            | None => Fail
           end
       end.
 
