theories/RTac/Assumption.v
@@ -6,7 +6,6 @@ Require Import MirrorCore.TypesI.
 Require Import MirrorCore.SubstI.
 Require Import MirrorCore.ExprDAs.
 Require Import MirrorCore.RTac.Core.
-Require Import MirrorCore.RTac.Open.
 
 Require Import MirrorCore.Util.Forwardy.
 
@@ -17,78 +16,41 @@ Section parameterized.
   Variable typ : Type.
   Variable expr : Type.
   Variable subst : Type.
-  Variable RType_typ : RType typ.
-  Variable Expr_expr : Expr RType_typ expr.
-  Variable Typ0_Prop : Typ0 _ Prop.
-  Variable Subst_subst : Subst subst expr.
-  Variable SubstOk_subst : @SubstOk _ _ _ _ Expr_expr Subst_subst.
-  Variable SubstUpdate_subst : SubstUpdate subst expr.
-  Variable SubstUpdateOk_subst : @SubstUpdateOk _ _ _ _ Expr_expr Subst_subst _ _.
 
-  Variable (check : expr -> expr -> subst -> option subst).
+  Context {RType_typ : RType typ}.
+  Context {Expr_expr : Expr RType_typ expr}.
+  Context {Typ0_Prop : Typ0 _ Prop}.
+  Context {Subst_subst : Subst subst expr}.
+  Context {SubstOk_subst : @SubstOk _ _ _ _ Expr_expr Subst_subst}.
+  Context {SubstUpdate_subst : SubstUpdate subst expr}.
+  Context {SubstUpdateOk_subst : @SubstUpdateOk _ _ _ _ Expr_expr Subst_subst _ _}.
+
+  Variable (check : Ctx typ expr -> expr -> expr -> subst -> option subst).
 
   Fixpoint findHyp s (ctx : Ctx typ expr) (g : expr) {struct ctx}
   : option subst :=
     match ctx with
       | CTop => None
-      | CAll t ctx' => findHyp s ctx' g
-      | CEx  t ctx' => findHyp s ctx' g
-      | CHyp h ctx' => match check g h s with
+      | CAll ctx' _ => findHyp s ctx' g
+      | CEx  ctx' _ => findHyp s ctx' g
+      | CHyp ctx' h => match check ctx' g h s with
                          | None => findHyp s ctx' g
                          | Some e => Some e
                        end
     end.
 
-  Fixpoint reduceGoal (ctx : Ctx typ expr) (s : subst) (un vn : nat)
-  : Ctx typ expr * subst :=
-    match ctx with
-      | CTop => (ctx, s)
-      | CAll l ctx' =>
-        match vn with
-          | 0 => (** STUCK **)
-            (ctx, s)
-          | S vn' =>
-            (** TODO: Drop var **)
-            reduceGoal ctx' s un vn'
-        end
-      | CEx  l ctx' =>
-        match un with
-          | 0 => (** STUCK **)
-            (ctx, s)
-          | S un' =>
-            match drop un' s with
-              | Some s' =>
-                reduceGoal ctx' s' un' vn
-              | None => (** STUCK **)
-                (ctx, s)
-            end
-        end
-      | CHyp h ctx' =>
-        reduceGoal ctx' s un vn
-    end.
-
-  Definition ASSUMPTION : rtac typ (expr) subst :=
-    fun g =>
-      let '(ctx,s,gl) := openGoal g in
-      match gl with
-        | None => Some g
-        | Some gl =>
-          match findHyp s ctx gl with
-            | None => None
-            | Some s' =>
-              let (tus,tvs) := getEnvs ctx in
-              let (ctx',s'') := reduceGoal ctx s' (length tus) (length tvs) in
-              Some (closeGoal ctx' (GGoal s'' None))
-          end
+  Definition ASSUMPTION : rtac typ expr subst :=
+    fun ctx s gl =>
+      match findHyp s ctx gl with
+        | None => Fail
+        | Some s' =>
+          Solved s'
       end.
-
-  Definition finish : rtac typ expr subst :=
-    fun g =>
-      let '(ctx,s,gl) := openGoal g in
-      let (tus,tvs) := getEnvs ctx in
-      let (ctx',s) := reduceGoal ctx s (length tus) (length tvs) in
-      Some (closeGoal ctx' (GGoal s None)).
 
   (** check soundness **)
 
 End parameterized.
+
+(*
+
+*)
