theories/RTac/EApply.v
@@ -5,11 +5,10 @@ Require Import MirrorCore.ExprI.
 Require Import MirrorCore.TypesI.
 Require Import MirrorCore.SubstI.
 Require Import MirrorCore.ExprDAs.
-Require Import MirrorCore.RTac.Core.
-Require Import MirrorCore.RTac.Continuation.
-Require Import MirrorCore.RTac.Open.
 Require Import MirrorCore.Lemma.
 Require Import MirrorCore.LemmaApply.
+Require Import MirrorCore.RTac.Core.
+Require Import MirrorCore.RTac.Reduce.
 
 Require Import MirrorCore.Util.Forwardy.
 
@@ -21,13 +20,13 @@ Section parameterized.
   Variable expr : Type.
   Variable subst : Type.
 
-  Variable RType_typ : RType typ.
-  Variable Expr_expr : Expr RType_typ expr.
-  Variable Typ0_Prop : Typ0 _ Prop.
-  Variable Subst_subst : Subst subst expr.
-  Variable SubstOk_subst : @SubstOk _ _ _ _ Expr_expr Subst_subst.
-  Variable SU : SubstUpdate subst expr.
-  Variable SubstUpdateOk_subst : @SubstUpdateOk _ _ _ _ Expr_expr Subst_subst _ _.
+  Context {RType_typ : RType typ}.
+  Context {Expr_expr : Expr RType_typ expr}.
+  Context {Typ0_Prop : Typ0 _ Prop}.
+  Context {Subst_subst : Subst subst expr}.
+  Context {SubstOk_subst : @SubstOk _ _ _ _ Expr_expr Subst_subst}.
+  Context {SU : SubstUpdate subst expr}.
+  Context {SubstUpdateOk_subst : @SubstUpdateOk _ _ _ _ Expr_expr Subst_subst _ _}.
 
   Variable vars_to_uvars : nat -> nat -> expr -> expr.
   Variable exprUnify : tenv typ -> tenv typ -> nat -> expr -> expr -> typ -> subst -> option subst.
@@ -39,54 +38,20 @@ Section parameterized.
 
   Definition EAPPLY
              (lem : Lemma.lemma typ expr expr)
-             (tacC : rtac_cont typ expr subst)
   : rtac typ expr subst :=
     let len_vars := length lem.(vars) in
-    fun gl =>
-      let '(ctx,sub,e) := openGoal gl in
+    fun ctx sub gl =>
       let '(tus,tvs) := getEnvs ctx in
-      match e with
-        | None => Some gl
-        | Some e =>
-          match eapplicable sub tus tvs lem e with
-            | None => None
-            | Some sub' =>
-              let len_uvars := length tus in
-              match pull (expr := expr) len_uvars len_vars sub' with
-                | Some sub'' =>
-                  (** If we have instantiated everything then we can be a little
-                   ** bit more efficient
-                   **)
-                  let premises :=
-                      map (fun e => instantiate (fun u => lookup u sub') 0
-                                                (vars_to_uvars 0 len_uvars e))
-                          lem.(premises)
-                  in
-                  tacC ctx sub'' premises
-                | None =>
-                  let premises := map (vars_to_uvars 0 len_uvars) lem.(premises) in
-                  tacC (fold_right (@CEx _ _) ctx lem.(vars)) sub' premises
-              (*
-              with
-                | None => None
-                | Solved tus' tvs' sub'' =>
-                  match pull (expr := expr) len_uvars len_vars sub'' with
-                    | None => @Fail _ _ _
-                    | Some sub''' => @Solved _ _ _ nil nil sub'''
-                  end
-                | More tus tvs sub'' hyps'' e =>
-                  (** TODO: In this case it is not necessary to pull everything
-                   ** I could leave unification variables in place
-                   **)
-                  match pull (expr := expr) len_uvars len_vars sub'' with
-                    | None => @Fail _ _ _
-                    | Some sub''' =>
-                      More (firstn len_uvars tus) tvs sub''' hyps'' e
-                  end
-              end
-               *)
-              end
-          end
+      match eapplicable sub tus tvs lem gl with
+        | None => Fail
+        | Some sub' =>
+          let len_uvars := length tus in
+          let premises := map (fun x => GGoal (vars_to_uvars 0 len_uvars x)) lem.(premises) in
+          reduceGoal instantiate (fold_left (@CEx _ _) lem.(vars) CTop) sub'
+                     match premises with
+                       | nil => GSolved
+                       | _ :: _ => GConj premises
+                     end (countUVars ctx + len_vars) (countVars ctx)
       end.
 
 End parameterized.
