theories/RTac/RTac.v
@@ -2,6 +2,7 @@ Require Export MirrorCore.RTac.Core.
 Require Export MirrorCore.RTac.Idtac.
 Require Export MirrorCore.RTac.Fail.
 Require Export MirrorCore.RTac.First.
+Require Export MirrorCore.RTac.Solve.
 Require Export MirrorCore.RTac.Then.
 Require Export MirrorCore.RTac.Try.
 Require Export MirrorCore.RTac.Repeat.
@@ -10,8 +11,11 @@ Require Export MirrorCore.RTac.RunSTac.
 Require Export MirrorCore.RTac.Intro.
 Require Export MirrorCore.RTac.Apply.
 Require Export MirrorCore.RTac.EApply.
-
+Require Export MirrorCore.RTac.Simplify.
+Require Export MirrorCore.RTac.Instantiate.
+Require Export MirrorCore.RTac.RunSTac.
 Require Export MirrorCore.RTac.AtGoal.
-
+(*
 Require Export MirrorCore.RTac.Continuation.
 Require Export MirrorCore.RTac.ApplyToAll.
+*)
