theories/RTac/Reduce.v
@@ -1,0 +1,103 @@
+Require Import ExtLib.Core.RelDec.
+Require Import ExtLib.Structures.Monad.
+Require Import ExtLib.Tactics.
+Require Import MirrorCore.EnvI.
+Require Import MirrorCore.ExprI.
+Require Import MirrorCore.TypesI.
+Require Import MirrorCore.SubstI.
+Require Import MirrorCore.ExprDAs.
+Require Import MirrorCore.InstantiateI.
+Require Import MirrorCore.RTac.Core.
+
+Require Import MirrorCore.Util.Forwardy.
+
+Set Implicit Arguments.
+Set Strict Implicit.
+
+Section parameterized.
+  Variable typ : Type.
+  Variable expr : Type.
+  Variable subst : Type.
+
+  Context {RType_typ : RType typ}.
+  Context {Expr_expr : Expr RType_typ expr}.
+  Context {Typ0_Prop : Typ0 _ Prop}.
+  Context {Subst_subst : Subst subst expr}.
+  Context {SubstOk_subst : @SubstOk _ _ _ _ Expr_expr Subst_subst}.
+  Context {SubstUpdate_subst : SubstUpdate subst expr}.
+  Context {SubstUpdateOk_subst : @SubstUpdateOk _ _ _ _ Expr_expr Subst_subst _ _}.
+
+  Variable instantiate : (nat -> option expr) -> nat -> expr -> expr.
+
+  Fixpoint instantiateGoal (f : nat -> option expr) (g : Goal typ expr)
+  : Goal typ expr :=
+    match g with
+      | GSolved => GSolved
+      | GGoal g => GGoal (instantiate f 0 g)
+      | GAll t g' => GAll t (instantiateGoal f g')
+      | GExs tes g' => GExs (List.map (fun te =>
+                                         match te with
+                                           | (t,None) => (t,None)
+                                           | (t,Some e) => (t,Some (instantiate f 0 e))
+                                         end) tes)
+                            (instantiateGoal f g')
+      | GHyp h g' => GHyp (instantiate f 0 h) (instantiateGoal f g')
+      | GConj ps =>
+        GConj (List.map (instantiateGoal f) ps)
+    end.
+
+  Fixpoint reduceGoal (ctx : Ctx typ expr) (s : subst) (g : Goal typ expr)
+           (un vn : nat)
+  : Result typ expr subst :=
+    match ctx with
+      | CTop => match g with
+                  | GSolved => Solved s
+                  | g => More s g
+                end
+      | CAll ctx' l =>
+        match vn with
+          | 0 => (** STUCK **)
+            Fail
+          | S vn' =>
+            (** TODO: Drop var **)
+            reduceGoal ctx' s g un vn'
+        end
+      | CEx  ctx' l =>
+        match un with
+          | 0 => (** STUCK **)
+            Fail
+          | S un' =>
+            match drop un' s with
+              | None =>
+                reduceGoal ctx' s (GEx l (lookup un' s) g) un' vn
+              | Some s' =>
+                match lookup un' s with
+                  | None => Fail (** DEAD **)
+                  | Some e =>
+                    (** NOTE: If this gets removed then all of the variables
+                     ** have to be renumbered. This is because this is
+                     ** actually a subst, not an instantiate
+                     **)
+                    let g' := instantiateGoal(fun u => if u ?[ eq ] un' then Some e else None) g
+                    in
+                    match g' with
+                      | GSolved =>
+                        reduceGoal ctx' s' g' un' vn
+                      | _ => reduceGoal ctx' s' (GEx l (Some e) g') un' vn
+                    end
+                end
+            end
+        end
+      | CHyp ctx' h =>
+        reduceGoal ctx' s g un vn
+    end.
+
+  Definition more_list (ctx : Ctx typ expr) (sub : subst)
+             (gl : list (Goal typ expr))
+  : Result typ expr subst :=
+    reduceGoal ctx sub match gl with
+                         | nil => GSolved
+                         | _ :: _ => GConj gl
+                       end (countUVars ctx) (countVars ctx).
+
+End parameterized.
