theories/RTac/Repeat.v
@@ -1,3 +1,4 @@
+(*Require Import Coq.PArith.BinPos. *)
 Require Import Coq.Lists.List.
 Require Import ExtLib.Core.RelDec.
 Require Import ExtLib.Structures.Monad.
@@ -13,6 +14,8 @@ Require Import MirrorCore.SubstI.
 Require Import MirrorCore.ExprDAs.
 Require Import MirrorCore.RTac.Core.
 Require Import MirrorCore.RTac.Try.
+Require Import MirrorCore.RTac.Idtac.
+Require Import MirrorCore.RTac.Then.
 
 Require Import MirrorCore.Util.Forwardy.
 
@@ -24,39 +27,37 @@ Section parameterized.
   Variable expr : Type.
   Variable subst : Type.
 
-  Variable RType_typ : RType typ.
-  Variable Expr_expr : Expr RType_typ expr.
-  Variable Typ0_Prop : Typ0 _ Prop.
-  Variable Subst_subst : Subst subst expr.
-  Variable SubstOk_subst : @SubstOk _ _ _ _ Expr_expr Subst_subst.
+  Context {RType_typ : RType typ}.
+  Context {Expr_expr : Expr RType_typ expr}.
+  Context {Typ0_Prop : Typ0 _ Prop}.
+  Context {Subst_subst : Subst subst expr}.
+  Context {SubstOk_subst : @SubstOk _ _ _ _ Expr_expr Subst_subst}.
+  Context {SubstUpdate_subst : SubstUpdate subst expr}.
 
+  (** TODO: Write this with a positive **)
   Section repeater.
-    Require Import Coq.PArith.BinPos.
+    (** TODO: To be efficient, this must be written in CPS
+     **)
+    Variable tac : rtac typ expr subst.
 
-    Fixpoint REPEAT' (n : positive) (tac : rtac typ expr subst)
-             {struct n}
+    Fixpoint REPEAT' (n : nat) {struct n}
     : rtac typ expr subst :=
-      fun gl =>
+      fun ctx sub gl =>
         match n with
-          | xH => tac gl
-          | xI n => match tac gl with
-                      | None => Some gl
-                      | Some gl' =>
-                        match REPEAT' n tac gl' with
-                          | None => Some gl'
-                          | Some gl'' => TRY (REPEAT' n tac) gl''
-                        end
-                    end
-          | xO n => match REPEAT' n tac gl with
-                      | None => Some gl
-                      | Some gl' => TRY (REPEAT' n tac) gl'
-                    end
+          | 0 => More sub (GGoal gl)
+          | S n =>
+            match tac ctx sub gl with
+              | Fail => More sub (GGoal gl)
+              | More sub' gl' =>
+                runRTac (REPEAT' n) ctx sub' gl'
+              | Solved s => Solved s
+            end
         end.
   End repeater.
 
   Definition REPEAT n (tac : rtac typ expr subst)
   : rtac typ expr subst :=
-    REPEAT' n tac.
+    REPEAT' tac n.
 
   Theorem REAPEAT_sound
   : forall tus tvs n tac, rtac_sound tus tvs tac ->
@@ -65,3 +66,39 @@ Section parameterized.
   Admitted.
 
 End parameterized.
+
+
+(*
+  Section repeater.
+    (** TODO: To be efficient, this must be written in CPS
+     **)
+    Variable tac : rtac typ expr subst.
+
+    Fixpoint REPEAT' (n : positive)
+             (onDone : Result typ expr subst -> Result typ expr subst)
+             (onContinue : Ctx typ expr -> subst -> Goal typ expr -> Result typ expr subst)
+             {struct n}
+    : Ctx typ expr -> subst -> expr -> Result typ expr subst :=
+      fun ctx sub gl =>
+        match n with
+          | xH => tac ctx sub gl
+          | xI n =>
+            match tac ctx sub gl with
+              | Fail => onDone (More sub (GGoal gl))
+              | More sub' gl' =>
+                runRTac (REPEAT' n onDone
+                                 (fun ctx' sub' gl' =>
+                                    runRTac (REPEAT' n onDone onContinue)
+                                            ctx' sub' gl'))
+                        ctx sub' gl'
+              | Solved s => onDone (Solved s)
+            end
+          | xO n =>
+            REPEAT' n onDone
+                    (fun ctx' sub' gl' =>
+                       runRTac (REPEAT' n onDone onContinue)
+                               ctx' sub' gl')
+           ctx sub gl
+        end.
+  End repeater.
+*)
