theories/RTac/Then.v
@@ -16,19 +16,33 @@ Section parameterized.
   Variable expr : Type.
   Variable subst : Type.
 
-  Variable RType_typ : RType typ.
-  Variable Expr_expr : Expr RType_typ expr.
-  Variable Typ0_Prop : Typ0 _ Prop.
-  Variable Subst_subst : Subst subst expr.
-  Variable SubstOk_subst : @SubstOk _ _ _ _ Expr_expr Subst_subst.
+  Context {RType_typ : RType typ}.
+  Context {Expr_expr : Expr RType_typ expr}.
+  Context {Typ0_Prop : Typ0 _ Prop}.
+  Context {Subst_subst : Subst subst expr}.
+  Context {SubstOk_subst : @SubstOk _ _ _ _ Expr_expr Subst_subst}.
+  Context {SubstUpdate_subst : SubstUpdate subst expr}.
+
+  (** c2 is put closer to the goal **)
+  Fixpoint Ctx_append (c1 c2 : Ctx typ expr) {struct c2} : Ctx typ expr :=
+    match c2 with
+      | CTop => c1
+      | CAll c2' t => CAll (Ctx_append c1 c2') t
+      | CEx  c2' t => CEx  (Ctx_append c1 c2') t
+      | CHyp c2' h => CHyp (Ctx_append c1 c2') h
+    end.
 
   Definition THEN (c1 c2 : rtac typ expr subst) : rtac typ expr subst :=
-    fun gl =>
-      match c1 gl with
-        | Some gl' => c2 gl'
-        | None => None
+    fun ctx sub g =>
+      match c1 ctx sub g with
+        | More sub' g' =>
+          runRTac c2 ctx sub' g'
+        | Solved sub =>
+          Solved sub
+        | Fail => Fail
       end.
 
+(*
   Theorem THEN_sound
   : forall (tus tvs : list typ) (tac1 tac2 : rtac typ expr subst),
       rtac_sound tus tvs tac1 ->
@@ -47,5 +61,5 @@ Section parameterized.
     split; auto.
     forward. eauto.
   Qed.
-
+*)
 End parameterized.
